var finished, doing abs

ML_SP_Inference.v
@@ -309,7 +309,7 @@ Lemma unify_type : forall K' S' h pairs K S,
   env_prop type S ->
   kenv_ok K ->
   (forall T1 T2, In (T1, T2) pairs -> type T1 /\ type T2) ->
-  kenv_ok K' /\ env_prop type S'.
+  kenv_ok K' /\ env_prop type S' /\ is_subst S'.
 Proof.
   induction h; simpl; intros. discriminate.
   destruct pairs. inversions* H.
@@ -733,14 +733,14 @@ Proof.
   intuition.
       destruct* (unify_keep _ _ _ HI).
     intro; intros.
-    apply H5.
+    apply H7.
     rewrite map_concat.
     apply* binds_concat_ok.
     rewrite <- map_concat.
     apply* ok_map0.
   rewrite <- (map_sch_subst_extend E Hext).
   use (unify_types _ _ _ HI HS0).
-  rewrite* <- (H6 (sch_open_vars s x) T).
+  rewrite* <- (H8 (sch_open_vars s x) T).
   rewrite* <- Hext.
   unfold fvs in f.
   rewrite* sch_subst_open_vars.
@@ -887,10 +887,10 @@ Proof.
     apply* well_subst_compose.
   use (unify_types _ _ _ R1 HS0).
   rewrite <- (H3 T).
-  rewrite* <- (H9 (typ_arrow (typ_fvar x) (typ_fvar x0)) T).
+  rewrite* <- (H11 (typ_arrow (typ_fvar x) (typ_fvar x0)) T).
   rewrite H3.
   simpl.
-  simpl map in H10.
+  simpl map in H11.
   fold (typ_subst S (typ_fvar x0)).
   fold (typ_subst S (typ_fvar x)).
   set (E' := map (sch_subst S) E) in *.
@@ -1736,7 +1736,8 @@ Qed.
 
 
 Definition principality S0 K0 S K E t T h :=
-  is_subst S0 -> kenv_ok K0 -> disjoint (dom S0) (dom K0) ->
+  is_subst S0 -> env_prop type S0 ->
+  kenv_ok K0 -> disjoint (dom S0) (dom K0) ->
   env_prop type S -> dom S << fvs S0 K0 E T -> extends S S0 ->
   well_subst (map (kind_subst S0) K0) K S ->
   K; map (sch_subst S) E |(false,GcAny)|= t ~: typ_subst S T ->
@@ -1748,125 +1749,158 @@ Definition principality S0 K0 S K E t T h :=
       extends (S & S'') S' /\
       well_subst (map (kind_subst S') K') K (S & S'').
 
-Theorem typinf_principal : forall S0 K0 S K E t T h,
-  principality S0 K0 S K E t T h.
+Lemma principal_var : forall h S0 K0 S K E x T,
+  principality S0 K0 S K E (trm_fvar x) T (Datatypes.S h).
 Proof.
-  intros; intros HS0 HK0 Dis HTS HS Hext WS Typ Hh.
-  gen_eq (map (sch_subst S) E) as E'.
-  gen_eq (typ_subst S T) as T'.
-  gen_eq (false,GcAny) as gc.
-  gen K0 S h.
-  induction Typ; intros; subst;
-    destruct h; try (simpl in Hh; elimtype False; omega).
-  (* Var *)
+  intros; intros HS0 HTS0 HK0 Dis HTS HS Hext WS Typ Hh.
+  inversions Typ; clear Typ; try discriminate.
   simpl.
-  destruct (binds_map_inv _ _ H1) as [M0 [HM0 B]].
+  destruct (binds_map_inv _ _ H5) as [M0 [HM0 B]].
   rewrite B.
   destruct (var_freshes (fvs S0 K0 E T) (sch_arity M0)) as [Xs Fr]; simpl.
-  case_eq
-    (unify (K0 & kinds_open_vars (sch_kinds M0) Xs) (sch_open_vars M0 Xs) T S0);
-    intros.
-  destruct p as [K' S']. esplit; esplit. split*.
-  unfold unify in H3.
   assert (AryM: sch_arity M0 = length Us).
-    destruct H2. subst. rewrite sch_arity_subst in H2.
-    apply (proj1 H2).
+    destruct H6. subst. rewrite sch_arity_subst in H.
+    apply (proj1 H).
   assert (Hsub: forall t, typ_fv t << fvs S0 K0 E T ->
                   typ_subst (S & combine Xs Us) t = typ_subst S t).
     rewrite AryM in Fr.
     intros.
     apply* typ_subst_combine_fresh.
     apply* fresh_sub.
-  unfold fvs in Fr.
   assert (Ok: ok (K0 & kinds_open_vars (sch_kinds M0) Xs)).
     apply* disjoint_ok. unfold kinds_open_vars. apply* ok_combine_fresh.
     rewrite* dom_kinds_open_vars.
-    apply disjoint_comm.
+    apply disjoint_comm. unfold fvs in Fr.
     apply* (fresh_disjoint (sch_arity M0)).
   assert (Hext': extends (S & combine Xs Us) S0).
     clear -Fr Hext Hsub.
-    apply* extends_concat. intros x Hx; auto with sets.
-  destruct* (unify_mgu0 (K':=K) (S':=S & combine Xs Us) _ H3).
-      subst.
-      unfold unifies; simpl; intros.
-      destruct* H5. inversions H5; clear H5.
-      destruct H2. rewrite sch_arity_subst in H2.
-      apply* unifies_open.
-      intros y Hy.
-      use (fv_in_spec sch_fv B).
-      destruct (S.union_1 Hy); auto with sets.
-    apply* well_subst_concat. subst*.
-  destruct* (unify_kinds_ok _ _ H3).
-    rewrite dom_concat.
-    rewrite* dom_kinds_open_vars.
-    disjoint_solve.
-  destruct H8.
-  exists (combine Xs Us).
-  split.
-    rewrite dom_combine.
+    apply* extends_concat. unfold fvs; intros x Hx; auto with sets.
+  assert (HU: unifies (S & combine Xs Us) ((sch_open_vars M0 Xs, T) :: nil)).
+    subst.
+    unfold unifies; simpl; intros.
+    destruct* H. inversions H; clear H.
+    destruct H6. rewrite sch_arity_subst in H.
+    apply* unifies_open.
     intros y Hy.
-    apply S.diff_3.
-Lemma unify_keep_fv : forall K S E T h pairs K0 S0,
-  Body.unify h pairs K0 S0 = Some (K, S) ->
-  fvs S0 K0 E T << fvs S K E T.
-Proof.
-  induction h; intros. discriminate.
-  simpl in H.
-  destruct pairs. inversions H; apply subset_refl.
-  destruct p.
-  case_rewrite (typ_subst S0 t) R1; case_rewrite (typ_subst S0 t0) R2.
-        destruct* (n === n0).
-        discriminate.
-       unfold unify_nv in H.
-       simpl in H. case_rewrite (S.mem v {}) R3.
-       case_rewrite (get_kind v K0) R4.
-       intros y Hy. apply* (IHh _ _ _ H).
-       unfold compose.
-       clear -Hy R4; unfold fvs in *.
-       rewrite dom_concat. rewrite dom_remove_env.
-       rewrite dom_map. rewrite fv_in_concat.
-       simpl dom.
-       destruct (S.union_1 Hy); clear Hy; auto with sets.
-       apply S.union_2.
-       destruct (S.union_1 H); clear H; auto with sets.
-       apply S.union_2.
-       destruct (y == v).
-         subst; auto 6 with sets.
-       union_solve y.
-Lemma fv_in_typ_subst : forall v T S,
-  fv_in typ_fv S << fv_in typ_fv (map (typ_subst (v ~ T)) S) \u {{v}}.
-Proof.
-  induction S; simpl; intros y Hy.  elim (in_empty Hy).
-  destruct a. simpl.
-  destruct (S.union_1 Hy); clear Hy.
-Lemma typ_fv_subst_keep : forall v T1 T,
-  typ_fv T << typ_fv (typ_subst (v ~ T1) T) \u {{v}}.
-Proof.
-  induction T; simpl; intros y Hy. elim (in_empty Hy).
-    destruct (v0 == v). subst. auto with sets.
-    simpl. auto with sets.
-  destruct (S.union_1 Hy); [use (IHT1 _ H) | use (IHT2 _ H)];
-    destruct (S.union_1 H0); auto with sets.
+    use (fv_in_spec sch_fv B).
+    destruct (S.union_1 Hy); unfold fvs; auto with sets.
+  case_eq
+    (unify (K0 & kinds_open_vars (sch_kinds M0) Xs) (sch_open_vars M0 Xs) T S0);
+    unfold unify; intros.
+    destruct p as [K' S']. esplit; esplit. split*.
+    unfold fvs in Fr.
+    destruct* (unify_mgu0 (K':=K) (S':=S & combine Xs Us) _ H).
+      apply* well_subst_concat. subst*.
+    destruct* (unify_kinds_ok _ _ H).
+      rewrite dom_concat.
+      rewrite* dom_kinds_open_vars.
+      disjoint_solve.
+    exists (combine Xs Us).
+    intuition.
+    rewrite dom_combine.
+      intros y Hy.
+      apply S.diff_3.
+        assert (y \in dom K' \u dom S').
+          apply H8.
+          rewrite dom_concat.
+          rewrite* dom_kinds_open_vars.
+          auto with sets.
+        unfold fvs; union_solve y.
+        auto 6 with sets.
+      destruct* (fresh_disjoint _ _ _ Fr y).
+    symmetry. rewrite* <- AryM.
+  elimtype False.
+  refine (unify_complete0 (K:=K) HS0 Ok Hext' HU _ _ H).
+    intro; intros.
+    rewrite <- (kind_subst_combine _ _ _ k Hext').
+    subst.
+    refine (well_subst_concat _ HTS HS H6 WS B Fr AryM Hsub Hext' _).
+    apply* binds_map.
+  omega.
 Qed.
-    destruct (S.union_1 (typ_fv_subst_keep v T _ H)); auto with sets.
-  destruct (S.union_1 (IHS _ H)); auto with sets.
+
+Lemma typ_subst_type' : forall S T,
+  type (typ_subst S T) -> type T.
+Proof.
+  induction T; simpl; intros; auto.
+  inversions H. auto.
 Qed.
-         use (fv_in_typ_subst v (typ_bvar n) _ H).
-         destruct (S.union_1 H0); auto 6 with sets.
-        rewrite
-    
-Search S.Subset.    
 
-
-    inversions 
-    rewrite <- kind_subst_compose.
-    destruct k as [[kc kv kr kh]|]; try apply wk_any.
-    simpl.
-    case_re
-  
-  
-     
-     
-
+Theorem typinf_principal : forall h S0 K0 S K E t T,
+  principality S0 K0 S K E t T h.
+Proof.
+  induction h; intros until T; intros HS0 HTS0 HK0 Dis HTS HS Hext WS Typ Hh;
+    try (elimtype False; omega).
+  inversions Typ.
+  apply* principal_var.
+  (* Abs *)
+  simpl.
+  destruct (var_fresh (fvs S0 K0 E T)) as [x1 Fr1]; simpl.
+  destruct (var_fresh (fvs S0 K0 E T \u {{x1}})) as [x2 Fr2]; simpl.
+  destruct (var_fresh (dom E \u trm_fv t1)) as [x Frx]; simpl.
+  pose (Xs := x1 :: x2 :: nil).
+  pose (Us := U :: T0 :: nil).
+  assert (Fr: fresh (fvs S0 K0 E T) 2 Xs) by simpl*.
+  assert (Hsub: forall t, typ_fv t << fvs S0 K0 E T ->
+                  typ_subst (S & combine Xs Us) t = typ_subst S t).
+    intros.
+    apply* typ_subst_combine_fresh.
+    apply* fresh_sub.
+  assert (Hext': extends (S & combine Xs Us) S0).
+    apply* extends_concat. unfold fvs; intros y Hy; auto with sets.
+  case_eq (unify K0 (typ_arrow (typ_fvar x1) (typ_fvar x2)) T S0);
+    unfold unify; intros.
+    destruct p as [K' S'].
+    destruct* (unify_mgu0 _ H1 (K':=K) (S':=S & combine Xs Us)).
+        intro; intros.
+        simpl in H2; destruct* H2. inversions H2; clear H2.
+        rewrite (typ_subst_combine_fresh S T2).
+          simpl. destruct* (x1 == x1).
+          destruct* (x2 == x1).
+            elim Fr2. rewrite e0. auto with sets.
+          destruct* (x2 == x2).
+        simpl length. unfold fvs in Fr. auto.
+      intro; intros.
+      destruct (binds_map_inv _ _ H2) as [k1 [Hk1 Bk1]].
+      subst k.
+      rewrite* (kind_subst_combine_fv (L:=fvs S0 K0 E T) S (S & combine Xs Us)).
+        rewrite <- (kind_subst_combine _ _ _ k1 Hext).
+        rewrite Hsub. apply* WS.
+        simpl; unfold fvs.
+        use (binds_dom Bk1).
+        intros y Hy. rewrite <- (S.singleton_1 Hy). auto 6 with sets.
+      intros. rewrite* Hext'.
+      unfold fvs.
+      use (fv_in_spec kind_fv Bk1).
+      eapply subset_trans; try apply H3.
+      intros y Hy; auto with sets.
+    destruct* (unify_type _ _ H1).
+      simpl; intros.
+      destruct* H5. inversions* H5.
+      split*. apply* (typ_subst_type' S).
+    destruct* (unify_kinds_ok _ _ H1).
+    destruct* (IHh S' K' (S & combine Xs Us) K ((x,Sch (typ_fvar x1) nil) :: E)
+                  (t1 ^ x) (typ_fvar x2)).
+            apply* env_prop_concat.
+            unfold Xs, Us.
+            intro; unfold binds; simpl; intros.
+            rewrite <- H in Typ.
+            use (proj44 (typing_regular Typ)).
+            inversions H10.
+            destruct (x0 == x1). inversion H9. rewrite* <- H12.
+            destruct (x0 == x2). inversion H9. rewrite* <- H12.
+            discriminate.
+          unfold fvs; simpl.
+          intros y Hy.
+          destruct (S.union_1 Hy); clear Hy.
+            unfold env_fv, sch_fv; simpl. auto with sets.
+          destruct (S.union_1 H9); clear H9.
+            auto with sets.
+          use (HS _ H10); clear H10.
+          unfold fvs, env_fv in H9.
+          unfold env_fv; simpl.
+          apply S.union_2.
+          union_solve y; auto 6 with sets.
+        
 End Mk2.
 End MkInfer.
